Veir/Rewriter/WellFormed/Rewriter/Operation.lean
@@ -5,406 +5,11 @@ import Veir.Rewriter.GetSetInBounds
 
 namespace Veir
 
-@[grind =]
-theorem OperationPtr.get!_linkBetween (op : OperationPtr)
-    (hneq : (nextOp = none ∧ prevOp = none) ∨ nextOp ≠ prevOp) (hnew : nextOp ≠ some self ∧ prevOp ≠ some self) (h₁ h₂ h₃) :
-    op.get! (linkBetween self ctx prevOp nextOp h₁ h₂ h₃) =
-    if op = self then
-      { op.get! ctx with prev := prevOp, next := nextOp }
-    else if prevOp = some op then
-      { op.get! ctx with next := self }
-    else if nextOp = some op then
-      { op.get! ctx with prev := self }
-    else
-      op.get! ctx := by
-  unfold linkBetween
-  split
-  · grind
-  · split <;> grind
-
-theorem OperationPtr.get!_linkBetweenWithParent (op : OperationPtr)
-    (hneq : (nextOp = none ∧ prevOp = none) ∨ nextOp ≠ prevOp) (hnew : nextOp ≠ some self ∧ prevOp ≠ some self) (h₁ h₂ h₃)
-    (heq : linkBetweenWithParent self ctx prevOp nextOp parent h₁ h₂ h₃ h₄ = some newCtx) :
-    op.get! newCtx =
-    if op = self then
-      { op.get! ctx with prev := prevOp, next := nextOp, parent := parent }
-    else if prevOp = some op then
-      { op.get! ctx with next := self }
-    else if nextOp = some op then
-      { op.get! ctx with prev := self }
-    else
-      op.get! ctx := by
-  sorry
-
-@[simp, grind →]
-theorem OperationPtr.get!_linkBetweenWithParent_same
-    (hneq : (nextOp = none ∧ prevOp = none) ∨ nextOp ≠ prevOp) (hnew : nextOp ≠ some self ∧ prevOp ≠ some self) (h₁ h₂ h₃)
-    (heq : linkBetweenWithParent self ctx prevOp nextOp parent h₁ h₂ h₃ h₄ = some newCtx) :
-    self.get! newCtx = { self.get! ctx with prev := prevOp, next := nextOp, parent := parent } := by
-  simp [OperationPtr.get!_linkBetweenWithParent (hneq := hneq) (hnew := hnew) (heq := heq)]
-
-@[grind =>]
-theorem OperationPtr.get!_linkBetweenWithParent_parent (op : OperationPtr)
-  (hneq : (nextOp = none ∧ prevOp = none) ∨ nextOp ≠ prevOp) (hnew : nextOp ≠ some self ∧ prevOp ≠ some self)
-  (heq : linkBetweenWithParent self ctx prevOp nextOp parent h₁ h₂ h₃ h₄ = some newCtx) :
-  (op.get! newCtx).parent =
-  if op = self then
-    some parent
-  else
-    (op.get! ctx).parent := by
-  rw [get!_linkBetweenWithParent _ hneq hnew (heq := heq)]
-  grind
-
-@[grind =>]
-theorem OperationPtr.get!_linkBetweenWithParent_prev (op : OperationPtr)
-  (hneq : (nextOp = none ∧ prevOp = none) ∨ nextOp ≠ prevOp) (hnew : nextOp ≠ some self ∧ prevOp ≠ some self)
-  (heq : linkBetweenWithParent self ctx prevOp nextOp parent h₁ h₂ h₃ h₄ = some newCtx) :
-  (op.get! newCtx).prev =
-  if op = self then
-    prevOp
-  else if nextOp = some op then
-    some self
-  else
-    (op.get! ctx).prev := by
-  rw [get!_linkBetweenWithParent _ hneq hnew (heq := heq)]
-  grind
-
-@[grind =>]
-theorem OperationPtr.get!_linkBetweenWithParent_next (op : OperationPtr)
-  (hneq : (nextOp = none ∧ prevOp = none) ∨ nextOp ≠ prevOp) (hnew : nextOp ≠ some self ∧ prevOp ≠ some self)
-  (heq : linkBetweenWithParent self ctx prevOp nextOp parent h₁ h₂ h₃ h₄ = some newCtx) :
-  (op.get! newCtx).next =
-  if op = self then
-    nextOp
-  else if prevOp = some op then
-    some self
-  else
-    (op.get! ctx).next := by
-  rw [get!_linkBetweenWithParent _ hneq hnew (heq := heq)]
-  grind
-
-@[simp, grind →]
-theorem OperationPtr.get!_linkBetweenWithParent_parent_same
-  (hneq : (nextOp = none ∧ prevOp = none) ∨ nextOp ≠ prevOp) (hnew : nextOp ≠ some self ∧ prevOp ≠ some self)
-  (heq : linkBetweenWithParent self ctx prevOp nextOp parent h₁ h₂ h₃ h₄ = some newCtx) :
-  (self.get! newCtx).parent = parent := by
-  grind
-
-@[simp, grind →]
-theorem OperationPtr.get_linkBetweenWithParent_parent_same
-  (hneq : (nextOp = none ∧ prevOp = none) ∨ nextOp ≠ prevOp) (hnew : nextOp ≠ some self ∧ prevOp ≠ some self)
-  (heq : linkBetweenWithParent self ctx prevOp nextOp parent h₁ h₂ h₃ h₄ = some newCtx) :
-  (self.get newCtx).parent = parent := by
-  grind
-
-@[simp]
-theorem OperationPtr.get!_linkBetweenWithParent_parent_other
-  (hneq : (nextOp = none ∧ prevOp = none) ∨ nextOp ≠ prevOp) (hnew : nextOp ≠ some self ∧ prevOp ≠ some self)
-  (heq : linkBetweenWithParent self ctx prevOp nextOp parent h₁ h₂ h₃ h₄ = some newCtx) (hnn : op ≠ self) :
-  (op.get! newCtx).parent = (op.get! ctx).parent := by
-  grind
-
-@[simp]
-theorem OperationPtr.get_linkBetweenWithParent_parent_other
-  (hneq : (nextOp = none ∧ prevOp = none) ∨ nextOp ≠ prevOp) (hnew : nextOp ≠ some self ∧ prevOp ≠ some self)
-  (heq : linkBetweenWithParent self ctx prevOp nextOp parent h₁ h₂ h₃ h₄ = some newCtx) (hnn : op ≠ self) :
-  (op.get newCtx).parent = (op.get ctx hop).parent := by
-  have := @OperationPtr.get!_linkBetweenWithParent_parent_other (heq := heq) (hneq := hneq) (hnew := hnew) (hnn := hnn)
-  grind
-
 @[grind]
 def InsertPoint.Wf (insertionPoint : InsertPoint) (ctx : IRContext) (newOp : OperationPtr) :=
   match insertionPoint with
   | before op => newOp ≠ op ∧ newOp ≠ (op.get! ctx).prev ∧ op ≠ (op.get! ctx).prev
   | atEnd bl => newOp ≠ (bl.get! ctx).lastOp
-
-theorem OperationPtr.get!_insertOp? {op : OperationPtr}
-    (hipWf : ip.Wf ctx newOp) (heq : Rewriter.insertOp? ctx newOp ip h₁ h₂ h₃ = some newCtx) :
-    op.get! newCtx =
-    match ip with
-    | .atEnd bl =>
-      if op = newOp then
-        { op.get! ctx with prev := (bl.get! ctx).lastOp, next := none, parent := some bl }
-      else if (bl.get! ctx).lastOp = some op then
-        { op.get! ctx with next := newOp }
-      else
-        op.get! ctx
-    | .before op' =>
-      if op = newOp then
-        { op.get! ctx with prev := (op'.get! ctx).prev, next := op', parent := (op'.get! ctx).parent }
-      else if op = op' then
-        { op.get! ctx with prev := .some newOp }
-      else if op = (op'.get! ctx).prev then
-        { op.get! ctx with next := .some newOp }
-      else
-        op.get! ctx := by
-  simp only [Rewriter.insertOp?] at heq
-  grind (splits := 25) [=> OperationPtr.get!_linkBetweenWithParent]
-
-theorem OperationPtr.get!_insertOp?_other (op : OperationPtr)
-    (hipWf : ip.Wf ctx newOp) (hother : ip.block! ctx ≠ (op.get! ctx).parent) (hnn : newOp ≠ op)
-    (heq : Rewriter.insertOp? ctx newOp ip h₁ h₂ h₃ = some newCtx) :
-    op.get! newCtx = op.get! ctx := by
-  rw [get!_insertOp? hipWf heq]
-  split
-  · simp
-    split
-    · simp_all
-    · split
-      · sorry -- need WF
-      · grind
-  · split
-    · simp_all
-    · split
-      · grind
-      · split
-        · simp_all [InsertPoint.block!]
-          sorry -- need WF
-        · grind
-
-@[grind =>]
-theorem OperationPtr.get!_insertOp?_parent (op : OperationPtr)
-    (hipWf : ip.Wf ctx newOp) (heq : Rewriter.insertOp? ctx newOp ip h₁ h₂ h₃ = some newCtx) :
-    (op.get! newCtx).parent =
-    if op = newOp then
-      ip.block! ctx
-    else
-      (op.get! ctx).parent := by
-  simp only [Rewriter.insertOp?] at heq
-  rw [get!_insertOp? hipWf heq] <;> grind
-
-@[simp, grind →]
-theorem OperationPtr.get!_insertOp?_parent_same
-    (hipWf : ip.Wf ctx newOp) (heq : Rewriter.insertOp? ctx newOp ip h₁ h₂ h₃ = some newCtx) :
-    (newOp.get! newCtx).parent = ip.block! ctx := by
-  grind
-
-@[simp, grind →]
-theorem OperationPtr.get_insertOp?_parent_same
-  (hipWf : ip.Wf ctx newOp) (heq : Rewriter.insertOp? ctx newOp ip h₁ h₂ h₃ = some newCtx) :
-  (newOp.get newCtx).parent = ip.block! ctx := by
-  grind
-
-@[simp]
-theorem OperationPtr.get!_insertOp?_parent_other
-    (hipWf : ip.Wf ctx newOp) (heq : Rewriter.insertOp? ctx newOp ip h₁ h₂ h₃ = some newCtx) (hnn : op ≠ newOp) :
-    (op.get! newCtx).parent = (op.get! ctx).parent := by
-  grind
-
-@[simp, grind =>]
-theorem OperationPtr.get!_insertOp?_operands {op : OperationPtr}
-    (hipWf : ip.Wf ctx newOp) (heq : Rewriter.insertOp? ctx newOp ip h₁ h₂ h₃ = some newCtx) :
-    (op.get! newCtx).operands = (op.get! ctx).operands := by
-  grind [OperationPtr.get!_insertOp? hipWf heq]
-
-@[simp, grind =>]
-theorem OperationPtr.get!_insertOp?_results {op : OperationPtr}
-    (hipWf : ip.Wf ctx newOp) (heq : Rewriter.insertOp? ctx newOp ip h₁ h₂ h₃ = some newCtx) :
-    (op.get! newCtx).results = (op.get! ctx).results := by
-  grind [OperationPtr.get!_insertOp? hipWf heq]
-
-@[simp, grind =>]
-theorem OperationPtr.getNumSuccessors!_insertOp? {op : OperationPtr}
-    (hipWf : ip.Wf ctx newOp) (heq : Rewriter.insertOp? ctx newOp ip h₁ h₂ h₃ = some newCtx) :
-    op.getNumSuccessors! newCtx = op.getNumSuccessors! ctx := by
-  sorry
-
-@[simp, grind =>]
-theorem OperationPtr.get!_insertOp?_regions {op : OperationPtr}
-    (hipWf : ip.Wf ctx newOp) (heq : Rewriter.insertOp? ctx newOp ip h₁ h₂ h₃ = some newCtx) :
-    (op.get! newCtx).regions = (op.get! ctx).regions := by
-  grind [OperationPtr.get!_insertOp? hipWf heq]
-
-@[simp, grind =>]
-theorem OperationPtr.get_insertOp?_other (op : OperationPtr) (hop : op.InBounds ctx)
-    (hipWf : ip.Wf ctx newOp) (hother : ip.block! ctx ≠ (op.get! ctx).parent) (hnn : newOp ≠ op)
-    (heq : Rewriter.insertOp? ctx newOp ip h₁ h₂ h₃ = some newCtx) :
-    op.get newCtx = op.get ctx hop := by
-  have := @get!_insertOp?_other
-  grind
-
-@[simp, grind =]
-theorem BlockPtr.get!_linkBetween (block : BlockPtr) h₁ h₂ h₃ :
-    block.get! (OperationPtr.linkBetween self ctx prevOp nextOp h₁ h₂ h₃) = block.get! ctx := by
-  unfold OperationPtr.linkBetween
-  grind
-
-@[simp, grind =]
-theorem RegionPtr.get!_linkBetween (region : RegionPtr) h₁ h₂ h₃ :
-    region.get! (OperationPtr.linkBetween self ctx prevOp nextOp h₁ h₂ h₃) = region.get! ctx := by
-  unfold OperationPtr.linkBetween
-  grind
-
-@[simp, grind .]
-theorem BlockOperandPtr.get!_insertOp? {blockOp : BlockOperandPtr}
-    (hipWf : ip.Wf ctx newOp) (heq : Rewriter.insertOp? ctx newOp ip h₁ h₂ h₃ = some newCtx) :
-    blockOp.get! newCtx = blockOp.get! ctx := by
-  sorry
-
-@[grind =>]
-theorem BlockPtr.get!_linkBetweenWithParent (block : BlockPtr) h₁ h₂ h₃ h₄
-    (heq : OperationPtr.linkBetweenWithParent self ctx prevOp nextOp parent h₁ h₂ h₃ h₄ = some newCtx) :
-    block.get! newCtx =
-    if parent = some block then
-      { block.get! ctx with firstOp := if prevOp.isSome then (block.get! ctx).firstOp else self,
-                            lastOp := if nextOp.isSome then (block.get! ctx).lastOp else self }
-    else
-      block.get! ctx := by
-  sorry -- TODO
-  -- simp only [OperationPtr.linkBetweenWithParent] at heq
-  -- split at heq
-  -- · grind
-  -- · split at heq
-  --   · split at heq
-  --     · grind
-  --     · grind
-  --   · split
-  --     · simp
-  --       split at heq
-  --       · grind
-  --       · simp_all
-  --         simp [BlockPtr.get!_OperationPtr_setParentWithCheck (by assumption)]
-  --     · grind
-
-@[grind =>]
-theorem BlockPtr.get_linkBetweenWithParent (block : BlockPtr) (hbl : block.InBounds ctx) h₁ h₂ h₃ h₄
-    (heq : OperationPtr.linkBetweenWithParent self ctx prevOp nextOp parent h₁ h₂ h₃ h₄ = some newCtx) :
-    block.get newCtx =
-    if parent = some block then
-      { block.get ctx hbl with firstOp := if prevOp.isSome then (block.get ctx hbl).firstOp else self,
-                               lastOp := if nextOp.isSome then (block.get ctx hbl).lastOp else self }
-    else
-      block.get ctx hbl := by
-  have := BlockPtr.get!_linkBetweenWithParent block h₁ h₂ h₃ h₄ (heq := heq)
-  grind
-
-@[grind =>]
-theorem RegionPtr.get!_linkBetweenWithParent (region : RegionPtr) h₁ h₂ h₃ h₄
-    (heq : OperationPtr.linkBetweenWithParent self ctx prevOp nextOp parent h₁ h₂ h₃ h₄ = some newCtx) :
-    region.get! newCtx = region.get! ctx := by
-  simp only [OperationPtr.linkBetweenWithParent] at heq
-  grind
-
-@[grind =>]
-theorem BlockPtr.get!_insertOp? (block : BlockPtr)
-    (hipWf : ip.Wf ctx newOp) (heq : Rewriter.insertOp? ctx newOp ip h₁ h₂ h₃ = some newCtx) :
-    block.get! newCtx =
-    match ip with
-    | .atEnd bl =>
-       if block = bl then
-         { block.get! ctx with lastOp := some newOp, firstOp := if (block.get! ctx).lastOp = none then some newOp else (block.get! ctx).firstOp }
-       else
-         block.get! ctx
-    | .before op' =>
-       if block = (op'.get! ctx).parent then
-         { block.get! ctx with firstOp := if (op'.get! ctx).prev = none then some newOp else (block.get! ctx).firstOp }
-       else
-         block.get! ctx := by
-  simp only [Rewriter.insertOp?] at heq
-  split at heq
-  · split at heq <;> rename_i existingOp hip
-    · grind
-    · split
-      · grind [OperationPtr.get!_linkBetweenWithParent]
-      · split
-        · simp
-          split
-          · grind [OperationPtr.get!_linkBetweenWithParent]
-          · simp at *
-            rw [BlockPtr.get!_linkBetweenWithParent (heq := heq)]
-            simp
-            rintro rfl
-            split
-            · congr
-            · simp at *
-              rw [OperationPtr.get!_eq_get (by grind)] at *
-              cases h : (existingOp.get ctx (by grind)).prev <;> grind
-        · grind [OperationPtr.get!_linkBetweenWithParent]
-  · split
-    · split
-      · simp [BlockPtr.get!_linkBetweenWithParent (heq := heq)]
-        split
-        · split
-          · grind
-          · rw [BlockPtr.get!_eq_get (by grind)]
-            cases h : (block.get ctx (by grind)).lastOp
-            · simp
-            · rename_i h1 _
-              exfalso
-              apply h1
-              simp_all
-        · grind
-      · grind
-    · grind
-
-@[grind .]
-theorem BlockPtr.get!_insertOp?_other (block : BlockPtr)
-    (hipWf : ip.Wf ctx newOp) (heq : Rewriter.insertOp? ctx newOp ip h₁ h₂ h₃ = some newCtx)
-    (hother : ip.block! ctx ≠ some block) :
-    block.get! newCtx = block.get! ctx := by
-  grind
-
- @[grind .]
-theorem BlockPtr.get_insertOp?_other (block : BlockPtr) (hblock : block.InBounds ctx)
-    (hipWf : ip.Wf ctx newOp) (heq : Rewriter.insertOp? ctx newOp ip h₁ h₂ h₃ = some newCtx)
-    (hother : ip.block! ctx ≠ some block) :
-    block.get newCtx = block.get ctx hblock := by
-  rw [← BlockPtr.get!_eq_get (by grind)]
-  grind
-
-@[grind =>]
-theorem BlockPtr.get!_insertOp?_firstuse (block : BlockPtr)
-    (hipWf : ip.Wf ctx newOp) (heq : Rewriter.insertOp? ctx newOp ip h₁ h₂ h₃ = some newCtx) :
-    (block.get! newCtx).firstUse = (block.get! ctx).firstUse := by
-  grind
-
-@[grind =>]
-theorem BlockPtr.get!_insertOp?_parent (block : BlockPtr)
-    (hipWf : ip.Wf ctx newOp) (heq : Rewriter.insertOp? ctx newOp ip h₁ h₂ h₃ = some newCtx) :
-    (block.get! newCtx).parent = (block.get! ctx).parent := by
-  grind
-
-@[grind =>]
-theorem BlockOperandPtr.get!_insertOp?_firstuse (block : BlockOperandPtr)
-    (hipWf : ip.Wf ctx newOp) (heq : Rewriter.insertOp? ctx newOp ip h₁ h₂ h₃ = some newCtx) :
-    block.get! newCtx = block.get! ctx := by
-  unfold Rewriter.insertOp? at heq
-  grind
-
-@[grind =>]
-theorem RegionPtr.get!_insertOp?_firstuse (region : RegionPtr)
-    (heq : Rewriter.insertOp? ctx newOp ip h₁ h₂ h₃ = some newCtx) :
-    region.get! newCtx = region.get! ctx := by
-  unfold Rewriter.insertOp? at heq
-  grind
-
-theorem OperationPtr.no_parent_of_get_insertBetweenWithParent_some
-    (hneq : (nextOp = none ∧ prevOp = none) ∨ nextOp ≠ prevOp) (hnew : nextOp ≠ some self ∧ prevOp ≠ some self)
-    (heq : OperationPtr.linkBetweenWithParent self ctx prevOp nextOp parent h₁ h₂ h₃ h₄ = some newCtx) :
-    (self.get ctx).parent = none := by
-  unfold OperationPtr.linkBetweenWithParent at heq
-  unfold OperationPtr.setParentWithCheck at heq
-  simp at heq
-  split at heq
-  · grind
-  · rename_i h
-    split at h
-    · grind
-    · rename_i h g
-      rw [← OperationPtr.get!_eq_get (by grind), get!_linkBetween] at g
-      all_goals grind
-
-theorem OperationPtr.no_parent_of_get_insertOp?_some
-    (hipWf : ip.Wf ctx newOp) (heq : Rewriter.insertOp? ctx newOp ip h₁ h₂ h₃ = some newCtx) :
-    (newOp.get ctx).parent = none := by
-  unfold Rewriter.insertOp? at heq
-  unfold InsertPoint.Wf at hipWf
-  split at heq
-  · split at heq
-    · grind
-    · simp at heq
-      apply no_parent_of_get_insertBetweenWithParent_some (heq := heq) <;> grind
-  · grind [no_parent_of_get_insertBetweenWithParent_some]
 
 /--
  - Get the index of the insertion point in the operation list of the block.
@@ -451,20 +56,10 @@ theorem InsertPoint.idxInOperationList_getElem? {op : OperationPtr} (hop : op.In
   have := this.allOpsInChain
   grind
 
-def InsertPoint.prev (ip : InsertPoint) (ctx : IRContext) : Option OperationPtr :=
-  match ip with
-  | before op => (op.get! ctx).prev
-  | atEnd block => (block.get! ctx).lastOp
-
-def InsertPoint.next (ip : InsertPoint) : Option OperationPtr :=
-  match ip with
-  | before op => op
-  | atEnd _ => none
-
 theorem InsertPoint.idxInOperationList_InsertPoint_prev_none
     (ipInBounds : ip.InBounds ctx) :
     InsertPoint.block ip ctx ipInBounds = some blockPtr →
-    (InsertPoint.prev ip ctx = none ↔
+    (InsertPoint.prev! ip ctx = none ↔
     InsertPoint.idxInOperationList ip ctx blockPtr blockInBounds ctxWf = 0) := by
   have ⟨array, harray⟩ := ctxWf.opChain blockPtr blockInBounds
   simp (disch := grind) only [BlockPtr.operationList_iff_BlockPtr_OperationChainWellFormed] at harray
@@ -472,10 +67,10 @@ theorem InsertPoint.idxInOperationList_InsertPoint_prev_none
   intro hblock
   cases ip
   case before op =>
-    simp_all only [idxInOperationList_Before, InsertPoint.block, InsertPoint.prev]
+    simp_all only [idxInOperationList_Before, InsertPoint.block, InsertPoint.prev!]
     grind [BlockPtr.OperationChainWellFormed]
   case atEnd bl =>
-    simp_all only [InsertPoint.block, InsertPoint.prev, InsertPoint.idxInOperationList]
+    simp_all only [InsertPoint.block, InsertPoint.prev!, InsertPoint.idxInOperationList]
     grind [BlockPtr.OperationChainWellFormed, Array.size_eq_zero_iff]
 
 theorem InsertPoint.next_idxInOperationList ctxWf ip :
@@ -485,62 +80,21 @@ theorem InsertPoint.next_idxInOperationList ctxWf ip :
 
 theorem InsertPoint.next_ne_firstOp (hWF : ctx.WellFormed) (ipInBounds : ip.InBounds ctx) :
     (BlockPtr.get blockPtr ctx blockInBounds).firstOp = some firstOp →
-    InsertPoint.prev ip ctx ≠ none →
+    InsertPoint.prev! ip ctx ≠ none →
     InsertPoint.next ip ≠ some firstOp
     := by
   intro hfirst hprev
   have ⟨array, harray⟩ := hWF.opChain blockPtr blockInBounds
   have := InsertPoint.next_idxInOperationList hWF ip harray
-  cases ip <;> grind [InsertPoint.prev, InsertPoint.next, BlockPtr.OperationChainWellFormed]
+  cases ip <;> grind [InsertPoint.prev!, InsertPoint.next, BlockPtr.OperationChainWellFormed]
 
 
 theorem InsertPoint.prev_idxInOperationList :
     let idx := InsertPoint.idxInOperationList ip ctx blockPtr blockInBounds ctxWf
     BlockPtr.OperationChainWellFormed blockPtr ctx array blockInBounds →
     idx > 0 →
-    ip.prev ctx = some array[idx - 1]! := by
+    ip.prev! ctx = some array[idx - 1]! := by
   sorry
-
-theorem BlockPtr.get!_insertOp?_firstOp
-    (hipWf : ip.Wf ctx newOp) (heq : Rewriter.insertOp? ctx newOp ip h₁ h₂ h₃ = some newCtx) :
-    (BlockPtr.get! block newCtx).firstOp =
-    if ip.block! ctx ≠ some block then
-      (block.get! ctx).firstOp
-    else if ip.prev ctx = none then
-        some newOp
-    else
-      (block.get! ctx).firstOp := by
-  sorry
-
-theorem OperationPtr.get!_insertOp?_prev {op : OperationPtr}
-    (hipWf : ip.Wf ctx newOp) (heq : Rewriter.insertOp? ctx newOp ip h₁ h₂ h₃ = some newCtx) :
-    (op.get! newCtx).prev =
-    if op ≠ newOp then
-      if ip.next = some op then
-        some newOp
-      else
-        (op.get! ctx).prev
-    else
-      ip.prev ctx
-    := by
-  have : (newOp.get ctx (by grind)).parent = none := by grind [OperationPtr.no_parent_of_get_insertOp?_some]
-  by_cases h: op = newOp
-  · subst op
-    simp only [ne_eq, not_true_eq_false, ↓reduceIte]
-    simp [OperationPtr.get!_insertOp? hipWf heq]
-    grind [InsertPoint.prev]
-  · simp [OperationPtr.get!_insertOp? hipWf heq]
-    grind [InsertPoint.next]
-
-theorem OperationPtr.get!_insertOp?_next {op : OperationPtr}
-    (hipWf : ip.Wf ctx newOp) (heq : Rewriter.insertOp? ctx newOp ip h₁ h₂ h₃ = some newCtx) :
-    (op.get! newCtx).next =
-    if op = newOp then ip.next else
-      if ip.prev ctx = some op then some newOp else (op.get! ctx).next := by
-  have : (newOp.get ctx (by grind)).parent = none := by grind [OperationPtr.no_parent_of_get_insertOp?_some]
-  by_cases h: op = newOp
-  · grind [OperationPtr.get!_insertOp? hipWf heq, InsertPoint.next]
-  · grind (splits := 20) [get!_insertOp? hipWf heq, InsertPoint.prev]
 
 @[grind .]
 theorem InsertPoint.idxInOperationList_Before_lt_size :
@@ -590,10 +144,40 @@ theorem InsertPoint.wf_insertOp?_isSome (hWF : ctx.WellFormed) {ipInBounds : ip.
 theorem BlockPtr.operationChainWellFormed_Rewriter_insertOp?_other
     (hol : BlockPtr.operationList blockPtr ctx ctxWellFormed blockInBounds = array)
     (hctx' : Rewriter.insertOp? ctx newOp ip newOpIn insIn ctxInBounds = some ctx')
-    (ipParent : InsertPoint.block ip ctx ipInBounds ≠ some blockPtr) :
+    (ipParent : InsertPoint.block! ip ctx ≠ some blockPtr) :
       blockPtr.OperationChainWellFormed ctx' array (by grind) := by
   have ipWf : ip.Wf ctx newOp := by rcases ip <;> grind
-  apply BlockPtr.OperationChainWellFormed_unchanged (ctx := ctx) <;> grind
+  apply BlockPtr.OperationChainWellFormed_unchanged (ctx := ctx) <;> try grind
+  · intros opPtr opInBounds opParent
+    simp only [OperationPtr.parent!_insertOp? hctx']
+    simp only [OperationPtr.prev!_insertOp? hctx']
+    simp only [OperationPtr.next!_insertOp? hctx']
+    constructor
+    · grind
+    · constructor
+      · grind
+      · constructor
+        · split
+          · simp_all [InsertPoint.block!, InsertPoint.next]
+            grind [BlockPtr.OperationChainWellFormed]
+          · grind
+        · split
+          · suffices (opPtr.get! ctx).parent = ip.block! ctx by grind
+            simp_all [InsertPoint.block!, InsertPoint.prev!]
+            cases ip
+            · rename_i op' _
+              simp_all only
+              cases hop'parent : (op'.get ctx).parent
+              · grind
+              · rename_i parent'
+                have ⟨array', harray'⟩ := ctxWellFormed.opChain parent' (by grind)
+                have : op' ∈ array' := by grind [IRContext.WellFormed, BlockPtr.OperationChainWellFormed]
+                have ⟨i, hi⟩ := Array.getElem?_of_mem this
+                have := harray'.prev i (by grind [IRContext.WellFormed, BlockPtr.OperationChainWellFormed]) (by grind)
+                grind [IRContext.WellFormed, BlockPtr.OperationChainWellFormed]
+            · simp_all only
+              grind [IRContext.WellFormed, BlockPtr.OperationChainWellFormed]
+          · grind
 
 theorem BlockPtr.operationChainWellFormed_Rewriter_insertOp?_self
     (hWf : BlockPtr.operationList blockPtr ctx ctxWellFormed blockInBounds = array)
@@ -615,31 +199,31 @@ theorem BlockPtr.operationChainWellFormed_Rewriter_insertOp?_self
     grind [BlockPtr.OperationChainWellFormed]
   case last =>
     simp only [Array.size_insertIdx, Nat.add_one_sub_one, Nat.lt_add_one, getElem?_pos]
-    simp [BlockPtr.get!_insertOp? blockPtr ipWf hctx']
+    simp [BlockPtr.lastOp!_insertOp? hctx']
+    simp_all [InsertPoint.block!, InsertPoint.next]
     cases hip: ip
     case before existingOp =>
       subst ip
-      simp only [InsertPoint.block!] at ipParent
-      simp only [ipParent, ↓reduceIte, InsertPoint.idxInOperationList_Before]
+      simp only [InsertPoint.idxInOperationList_Before]
       rw [Array.getElem_insertIdx_of_gt] <;> grind [BlockPtr.OperationChainWellFormed]
     case atEnd => grind [InsertPoint.idxInOperationList]
   case prevFirst =>
     intros firstOp hFirstOp
-    simp only [←BlockPtr.get!_eq_get] at hFirstOp
-    simp (disch := grind) only [BlockPtr.get!_insertOp?_firstOp ipWf hctx'] at hFirstOp
-    simp only [ipParent, ne_eq, not_true_eq_false, ↓reduceIte] at hFirstOp
+    simp only [BlockPtr.firstOp!_insertOp? hctx'] at hFirstOp
+    simp only [ipParent, true_and] at hFirstOp
     split at hFirstOp
     case isTrue =>
       simp only [Option.some.injEq] at hFirstOp
       subst firstOp
-      simp only [←OperationPtr.get!_eq_get, OperationPtr.get!_insertOp?_prev ipWf hctx']
+      simp only [OperationPtr.prev!_insertOp? hctx', ↓reduceIte]
+      simp_all only [InsertPoint.Wf, InsertPoint.next]
       grind
     case isFalse ipprev =>
-      simp only [←OperationPtr.get!_eq_get, OperationPtr.get!_insertOp?_prev ipWf hctx']
+      simp only [OperationPtr.prev!_insertOp? hctx']
       grind [InsertPoint.next_ne_firstOp, BlockPtr.OperationChainWellFormed]
   case allOpsInChain =>
     intros op opInBounds opParent
-    simp only [←OperationPtr.get!_eq_get, OperationPtr.get!_insertOp?_parent op ipWf hctx'] at opParent
+    simp only [←OperationPtr.get!_eq_get, OperationPtr.parent!_insertOp? hctx'] at opParent
     simp [Array.mem_insertIdx]
     split at opParent
     · grind
@@ -651,9 +235,8 @@ theorem BlockPtr.operationChainWellFormed_Rewriter_insertOp?_self
     · have : op.InBounds ctx := by grind [BlockPtr.OperationChainWellFormed]
       grind
   case first =>
-    simp only [←BlockPtr.get!_eq_get, BlockPtr.get!_insertOp?_firstOp ipWf hctx']
-    simp only [ipParent, ne_eq, not_true_eq_false, ↓reduceIte, Array.size_insertIdx,
-      Nat.zero_lt_succ, getElem?_pos]
+    simp only [BlockPtr.firstOp!_insertOp? hctx']
+    simp only [ipParent, true_and, Array.size_insertIdx, Nat.zero_lt_succ, getElem?_pos]
     have := InsertPoint.idxInOperationList_InsertPoint_prev_none ipInBounds (ctxWf := ctxWellFormed) (blockPtr := blockPtr) (blockInBounds := by grind)
     split
     case isTrue => grind
@@ -667,7 +250,7 @@ theorem BlockPtr.operationChainWellFormed_Rewriter_insertOp?_self
     simp only [gt_iff_lt, Array.size_insertIdx]
     intros i h₁ h₂
     let idx := ip.idxInOperationList ctx blockPtr blockInBounds ctxWellFormed
-    simp [OperationPtr.get!_insertOp?_prev ipWf hctx']
+    simp [OperationPtr.prev!_insertOp? hctx']
     have idxInBounds := @InsertPoint.idxInOperationList_inBounds ip ctx blockPtr (by grind) (by grind)
     simp only [hWf] at idxInBounds
     by_cases hi : i < idx
@@ -681,6 +264,7 @@ theorem BlockPtr.operationChainWellFormed_Rewriter_insertOp?_self
     · subst i idx
       simp only [Array.getElem_insertIdx_self, ↓reduceIte]
       simp (disch := grind) [Array.getElem_insertIdx_of_lt]
+      simp_all only [InsertPoint.Wf, InsertPoint.next]
       have := @InsertPoint.prev_idxInOperationList
       grind
     by_cases hi'' : i = idx + 1
@@ -697,14 +281,18 @@ theorem BlockPtr.operationChainWellFormed_Rewriter_insertOp?_self
       suffices ip.next ≠ some array[i - 1] by grind [BlockPtr.OperationChainWellFormed]
       grind [BlockPtr.OperationChainWellFormed_array_injective]
   case next =>
-    simp only [Array.size_insertIdx, ←OperationPtr.get!_eq_get]
+    simp only [Array.size_insertIdx]
     intros i hi
     let idx := ip.idxInOperationList ctx blockPtr blockInBounds ctxWellFormed
-    simp [OperationPtr.get!_insertOp?_next ipWf hctx']
+    simp only [OperationPtr.next!_insertOp? hctx']
     have idxInBounds := @InsertPoint.idxInOperationList_inBounds ip ctx blockPtr (by grind) (by grind)
     simp only [hWf] at idxInBounds
     by_cases hi' : i = idx
-    · grind [InsertPoint.next_idxInOperationList]
+    · subst i
+      rw [Array.getElem_insertIdx_self]
+      simp only [↓reduceIte]
+      have : some newOp ≠ ip.prev! ctx := by simp_all [InsertPoint.Wf, InsertPoint.prev!]; grind
+      grind [InsertPoint.next_idxInOperationList]
     by_cases hi'' : i + 1 = idx
     · simp (disch := grind) only [Array.getElem_insertIdx_of_lt]
       have : idx = i + 1 := by grind
@@ -716,14 +304,14 @@ theorem BlockPtr.operationChainWellFormed_Rewriter_insertOp?_self
     · simp (disch := grind) only [Array.getElem_insertIdx_of_gt]
       have : array[i-1]? ≠ some newOp := by grind [BlockPtr.OperationChainWellFormed]
       simp only [Array.getElem_eq_iff, this, ↓reduceIte]
-      suffices ip.prev ctx ≠ some array[i - 1] by grind [BlockPtr.OperationChainWellFormed]
+      suffices ip.prev! ctx ≠ some array[i - 1] by grind [BlockPtr.OperationChainWellFormed]
       by_cases idx = 0
       · rcases ip
         · have := hOCWF.first
-          grind [@hOCWF.prevFirst array[0] (by grind), InsertPoint.prev]
+          grind [@hOCWF.prevFirst array[0] (by grind), InsertPoint.prev!]
         · grind
       rcases ip with ⟨op⟩ | _
-      · simp [InsertPoint.prev]
+      · simp [InsertPoint.prev!]
         have : (array[idx].get! ctx).prev = some array[idx - 1] := by
           apply BlockPtr.OperationChainWellFormed.prev hOCWF; grind
         grind [BlockPtr.OperationChainWellFormed_array_injective]
@@ -732,8 +320,8 @@ theorem BlockPtr.operationChainWellFormed_Rewriter_insertOp?_self
       simp (disch := grind) only [Array.getElem_insertIdx_of_lt]
       have : array[i]? ≠ some newOp := by grind [BlockPtr.OperationChainWellFormed]
       simp only [Array.getElem_eq_iff, this, ↓reduceIte]
-      have : ip.prev ctx = some array[idx-1]! := by grind [InsertPoint.prev_idxInOperationList]
-      suffices ip.prev ctx ≠ some array[i] by grind [BlockPtr.OperationChainWellFormed]
+      have : ip.prev! ctx = some array[idx-1]! := by grind [InsertPoint.prev_idxInOperationList]
+      suffices ip.prev! ctx ≠ some array[i] by grind [BlockPtr.OperationChainWellFormed]
       grind [BlockPtr.OperationChainWellFormed_array_injective]
 
 theorem BlockPtr.operationList_Rewriter_insertOp?
@@ -750,19 +338,6 @@ theorem BlockPtr.operationList_Rewriter_insertOp?
     grind [BlockPtr.operationChainWellFormed_Rewriter_insertOp?_self]
   · simp only [←BlockPtr.operationList_iff_BlockPtr_OperationChainWellFormed]
     grind [BlockPtr.operationChainWellFormed_Rewriter_insertOp?_other]
-
-@[grind =>]
-theorem OpOperandPtr.get!_insertOp?
-    (hctx' : Rewriter.insertOp? ctx newOp ip newOpIn insIn ctxInBounds = some ctx') (opr: OpOperandPtr) :
-    opr.get! ctx' = opr.get! ctx := by
-  simp only [Rewriter.insertOp?] at hctx'
-  grind
-
-@[grind =>]
-theorem OperationPtr.getNumOperands!_insertOp?
-    (hctx' : Rewriter.insertOp? ctx newOp ip newOpIn insIn ctxInBounds = some ctx') (op: OperationPtr) :
-    op.getNumOperands! ctx' = op.getNumOperands! ctx := by
-  sorry -- We are missing some lemmas to do this
 
 theorem Rewriter.insertOp?_WellFormed (ctx : IRContext) (hctx : ctx.WellFormed)
     (newOp : OperationPtr) (ip : InsertPoint)
